common/Builtins.v
@@ -1,0 +1,58 @@
+(* *********************************************************************)
+(*                                                                     *)
+(*              The Compcert verified compiler                         *)
+(*                                                                     *)
+(*          Xavier Leroy, Collège de France and Inria Paris            *)
+(*                                                                     *)
+(*  Copyright Institut National de Recherche en Informatique et en     *)
+(*  Automatique.  All rights reserved.  This file is distributed       *)
+(*  under the terms of the GNU General Public License as published by  *)
+(*  the Free Software Foundation, either version 2 of the License, or  *)
+(*  (at your option) any later version.  This file is also distributed *)
+(*  under the terms of the INRIA Non-Commercial License Agreement.     *)
+(*                                                                     *)
+(* *********************************************************************)
+
+(** Known built-in functions *)
+
+Require Import String Coqlib.
+Require Import AST Integers Floats Values.
+Require Export Builtins0 Builtins1.
+
+Inductive builtin_function : Type :=
+  | BI_standard (b: standard_builtin)
+  | BI_platform (b: platform_builtin).
+
+Definition builtin_function_sig (b: builtin_function) : signature :=
+  match b with
+  | BI_standard b => standard_builtin_sig b
+  | BI_platform b => platform_builtin_sig b
+  end.
+
+Definition builtin_function_sem (b: builtin_function) : builtin_sem (proj_sig_res (builtin_function_sig b)) :=
+  match b with
+  | BI_standard b => standard_builtin_sem b
+  | BI_platform b => platform_builtin_sem b
+  end.
+
+Definition lookup_builtin_function (name: string) (sg: signature) : option builtin_function :=
+  match lookup_builtin standard_builtin_sig name sg standard_builtin_table with
+  | Some b => Some (BI_standard b)
+  | None => 
+  match lookup_builtin platform_builtin_sig name sg platform_builtin_table with
+  | Some b => Some (BI_platform b)
+  | None => None
+  end end.
+
+Lemma lookup_builtin_function_sig:
+  forall name sg b, lookup_builtin_function name sg = Some b -> builtin_function_sig b = sg.
+Proof.
+  unfold lookup_builtin_function; intros.
+  destruct (lookup_builtin standard_builtin_sig name sg standard_builtin_table) as [bs|] eqn:E.
+  inv H. simpl. eapply lookup_builtin_sig; eauto.
+  destruct (lookup_builtin platform_builtin_sig name sg platform_builtin_table) as [bp|] eqn:E'.
+  inv H. simpl. eapply lookup_builtin_sig; eauto.
+  discriminate.
+Qed.
+
+
