x86/Builtins1.v
@@ -1,0 +1,54 @@
+(* *********************************************************************)
+(*                                                                     *)
+(*              The Compcert verified compiler                         *)
+(*                                                                     *)
+(*          Xavier Leroy, Collège de France and Inria Paris            *)
+(*                                                                     *)
+(*  Copyright Institut National de Recherche en Informatique et en     *)
+(*  Automatique.  All rights reserved.  This file is distributed       *)
+(*  under the terms of the GNU General Public License as published by  *)
+(*  the Free Software Foundation, either version 2 of the License, or  *)
+(*  (at your option) any later version.  This file is also distributed *)
+(*  under the terms of the INRIA Non-Commercial License Agreement.     *)
+(*                                                                     *)
+(* *********************************************************************)
+
+(** Platform-specific built-in functions *)
+
+Require Import String Coqlib.
+Require Import AST Integers Floats Values.
+Require Import Builtins0.
+
+Inductive platform_builtin : Type :=
+  | BI_fmin
+  | BI_fmax.
+
+Local Open Scope string_scope.
+
+Definition platform_builtin_table : list (string * platform_builtin) :=
+     ("__builtin_fmin", BI_fmin)
+  :: ("__builtin_fmax", BI_fmax)
+  :: nil.
+
+Definition platform_builtin_sig (b: platform_builtin) : signature :=
+  match b with
+  | BI_fmin | BI_fmax =>
+      mksignature (Tfloat :: Tfloat :: nil) (Some Tfloat) cc_default
+  end.
+
+Definition platform_builtin_sem (b: platform_builtin) : builtin_sem (proj_sig_res (platform_builtin_sig b)) :=
+  match b with
+  | BI_fmin =>
+      mkbuiltin_n2t Tfloat Tfloat Tfloat
+        (fun f1 f2 => match Float.compare f1 f2 with
+                      | Some Eq | Some Lt => f1
+                      | Some Gt | None => f2
+                      end)
+  | BI_fmax =>
+      mkbuiltin_n2t Tfloat Tfloat Tfloat
+        (fun f1 f2 => match Float.compare f1 f2 with
+                      | Some Eq | Some Gt => f1
+                      | Some Lt | None => f2
+                      end)
+  end.
+
